Weak_Traces.thy
@@ -1,0 +1,53 @@
+theory Weak_Traces
+  imports Main HML_SRBB Expressiveness_Price
+begin
+
+inductive
+      is_trace_formula :: "('act, 'i) hml_srbb \<Rightarrow> bool"
+  and is_trace_formula_conjunction :: "('act, 'i) hml_srbb_conjunction \<Rightarrow> bool" where
+  "is_trace_formula TT" |
+  "is_trace_formula (Internal \<chi>)" if "is_trace_formula_conjunction \<chi>" |
+  "is_trace_formula_conjunction (Obs \<alpha> \<phi>)" if "is_trace_formula \<phi>"
+
+lemma trace_formula_to_expressiveness:
+  fixes \<phi> :: "('act, 'i) hml_srbb"
+  fixes \<chi> :: "('act, 'i) hml_srbb_conjunction"
+  shows  "(is_trace_formula \<phi>             \<longrightarrow> (\<phi> \<in> \<O> (E \<infinity> 0 0 0 0 0 0 0)))
+        \<and> (is_trace_formula_conjunction \<chi> \<longrightarrow> (\<chi> \<in> \<O>_\<chi> (E \<infinity> 0 0 0 0 0 0 0)))"
+  apply (rule is_trace_formula_is_trace_formula_conjunction.induct)
+  by (simp add: \<O>_def \<O>_\<chi>_def leq_not_eneg)+
+
+lemma expressiveness_to_trace_formula:
+  fixes \<phi> :: "('act, 'i) hml_srbb"
+  fixes \<chi> :: "('act, 'i) hml_srbb_conjunction"
+  shows "(\<phi> \<in> \<O> (E \<infinity> 0 0 0 0 0 0 0) \<longrightarrow> is_trace_formula \<phi>)
+       \<and> (\<chi> \<in> \<O>_\<chi> (E \<infinity> 0 0 0 0 0 0 0) \<longrightarrow> is_trace_formula_conjunction \<chi>) 
+       \<and> True"
+  apply (rule hml_srbb_hml_srbb_conjunction_hml_srbb_conjunct.induct)
+  using is_trace_formula_is_trace_formula_conjunction.intros(1) apply blast
+  apply (simp add: \<O>_\<chi>_def \<O>_def is_trace_formula_is_trace_formula_conjunction.intros(2))
+  apply (simp add: \<O>_def leq_not_eneg)
+  by (simp add: \<O>_\<chi>_def \<O>_def is_trace_formula_is_trace_formula_conjunction.intros(3) leq_not_eneg)+
+
+lemma modal_depth_only_is_trace_form: 
+  "(is_trace_formula \<phi>) = (\<phi> \<in> \<O> (E \<infinity> 0 0 0 0 0 0 0))"
+  using expressiveness_to_trace_formula trace_formula_to_expressiveness by blast
+
+context Inhabited_Tau_LTS
+begin
+
+lemma
+  fixes \<phi> :: "('a, 's) hml_srbb"
+  fixes \<chi> :: "('a, 's) hml_srbb_conjunction"
+  fixes \<psi> :: "('a, 's) hml_srbb_conjunct"
+  shows "(is_trace_formula \<phi> \<longrightarrow> (\<phi> \<Turnstile>SRBB p \<longrightarrow> \<phi> \<Turnstile>SRBB q))
+      \<and> (is_trace_formula_conjunction \<chi> \<longrightarrow> (hml_srbb_conjunction_models \<chi> p \<longrightarrow> hml_srbb_conjunction_models \<chi> q))
+      \<and> (\<lambda>x. True) \<psi>"
+  sorry
+
+lemma "(p \<lesssim>WT q) = (p \<preceq> (E \<infinity> 0 0 0 0 0 0 0) q)"
+  sorry
+
+end
+
+end
